%----PrefaceImport----%
\documentclass{article}
\usepackage{fancyhdr}
\usepackage[a4paper,margin=1in,headsep=25pt]{geometry}
\usepackage{lipsum,hyperref}
\usepackage{enumerate,fullpage,proof}
\usepackage[fontsize=12pt]{fontsize}
\usepackage{amsmath,amscd,amsbsy,amssymb,latexsym,url,bm,amsthm}
\usepackage{epsfig,graphicx,subfigure}
\usepackage[usenames]{xcolor}

\newtheorem{thm}{Theorem}
\newtheorem{lemma}[thm]{Lemma}

\pagestyle{fancy}
\pagenumbering{Alph}
\setlength{\headheight}{36.0pt}
\headsep = 25pt
\fancyhf{}
\lhead{CSE 3302/5307 Programming Language Concepts}
\rhead{Homework3:Untyped Lambda Calculus}
\lfoot{2023 Kenny Zhu}
%----Documentation----%
\begin{document}

\title{CSE 3302/5307 Programming Language Concepts}
\author{Homework3 - Fall 2023}
\date{Due Date: Sep.16, 2023, 8:00p.m. Central Time}
\maketitle
\thispagestyle{fancy}

%----Homeworks----%

\section*{Problem1 - 40\%}

Evaluate the following $\lambda$ expressions using call-by-value and call-by-name. Show the complete steps of evaluation.
\begin{enumerate}[(a)]
    \item $(\lambda x.\ ((\lambda y.\ x+z+3 )\ 3 )5)$
    \item $((\lambda v.(\lambda w.w))\ ((\lambda x.x)\ (y\ (\lambda z.z))))$
    \item $((\lambda x.\ x\ x)\ (\lambda y.\ y\ y))$
    \item $((\lambda x. \lambda y. x)\ (\lambda z.z\ \lambda u.u))$
\end{enumerate}

\section*{Problem2 - 30\%}

Prove by induction: If $e_{1}$ is closed and $e_{1} \rightarrow e_{2}$, then $e_{2}$ is closed.
Suppose using call by value evaluation. 
\begin{itemize}
\item Given the following definitions:
\begin{enumerate}
    \item Rules of free variables (You can use these rules directly without writing "By ...")
    \[
    \frac{}{FV(x)=\{x\}} \qquad
    \frac{FV(e_1) = S_1\quad FV(e_2) = S_2}{FV(e_1\ e_2)=S_1\cup S_2} \qquad
    \frac{FV(e) = S}{FV(\\x.e)=S-\{x\}}
    \]
    \item Judgment form: \textbf{define} $e_1\rightarrow e_2$
    \[
    \frac{}{(\lambda x.e)\ v \rightarrow e [v/x]}
    \qquad
    \frac{e_1 \rightarrow e_1^{'}}{e_1\ e_2 \rightarrow e_1^{'}\ e_2}
    \qquad
    \frac{e_2 \rightarrow e_2^{'}}{v\ e_2 \rightarrow v\ e_2^{'}}
    \]
    
    \item Judgment form: \textbf{define} $e_1{\rightarrow}^*e_2$
    \[
    \frac{}{e_1\rightarrow^* e_1}
    \qquad
    \frac{e_1\rightarrow e_2\qquad e_2\rightarrow^*e_3}{e_1\rightarrow^*e_3}
    \]
\end{enumerate}
\newpage
\item And given this lemma:
    \begin{lemma}\label{fv}
        $FV(e_1[e_2/x]) \subseteq (FV(e_1) - \{x\}) \cup FV(e_2)$
    \end{lemma}
You can use this lemma directly. (Proof is in the appendix)
\end{itemize}
\vspace{20pt}
\section*{Problem3 - 30\%}

Church encoding is a means of embedding data and operators into the $\lambda$ calculus, the most familiar form being the Church numerals, a representation of the natural numbers using $\lambda$ notation. 
Church numerals $\mathbf{0}, \mathbf{1}, \mathbf{2}, ...,$ are defined as follows:
\begin{align*}
    \mathbf{0} &= \lambda f.\lambda x.\ x \\
    \mathbf{1} &= \lambda f.\lambda x.\ f\ x \\
    \mathbf{2} &= \lambda f.\lambda x.\ f\ (f\ x) \\
    \mathbf{3} &= \lambda f.\lambda x.\ f\ (f\ (f\ x)) \\
    &\dots \\
    \mathbf{n} &= \lambda f.\lambda x.\ f^n\ x \\
    &\dots
\end{align*}
Church numerals takes two parameters $f$ and $x$. Church numerals $n$ means apply $f$ to $x$ $n$ times.
(You can refer to Wikipedia or other references about Church encoding to know more about the idea of church encoding)
\begin{enumerate}[(a)]
    \item Define addition in $\lambda$ calculus, and then show the evaluation of $3+2$.
    \item Define multiplication in $\lambda$ calculus (Hint: use definition of addition), and then show the evaluation of $3\times2$.
    \item Give a definition of multiplication on Church numerals without using addition.
\end{enumerate}

\vspace{20pt}

\textbf{Remark:} 

Please email \textbf{.pdf} files to TA.

File name format: {\color{red} HW\_X\_FirstName\_10digitID.pdf}

Example: {HW\_3\_Sinong\_1001001000.pdf}

\newpage

\appendix
\renewcommand{\appendixname}{Appendix~\Alph{section}}

\section{Proof of Lemma 1}


\textbf{Lemma}	$FV(e_1[e/x]) \subseteq (FV(e_1) - \{x\}) \cup FV(e)$


\begin{proof}
	By induction on the derivation of substitution. (Actually you can treat substitution as a special judgement form and the definitions as rules)
	\begin{enumerate}
		\item case $x[e/x] = e$
		
		Need to prove: $FV(x[e/x]) \subseteq (FV(x)-\{x\}) \cup FV(e)$
		
		(1) $FV(x[e/x])=FV(e)$ (by assumption)
		
		(2) $FV(e) \subseteq (FV(x) - \{x\}) \cup FV(e)$
		
		(3) $FV(x[e/x]) \subseteq (FV(x)-\{x\}) \cup FV(e)$ (by (1) and (2))
		
		\item case $y[e/x] = y$
		
		Need to prove: $FV(y[e/x]) \subseteq (FV(y)-\{x\}) \cup FV(e)$
		
		(1) $FV(y[e/x])=FV(y)$ (by assumption)
		
		(2) $FV(y) \subseteq FV(y)-\{x\} \subseteq (FV(y)-\{x\}) \cup FV(e)$
		
		(3) $FV(y[e/x]) \subseteq (FV(y)-\{x\}) \cup FV(e)$ (by (1) and (2))
		
		\item case $(e_1\ e_2)[e/x] = e_1[e/x]\ e_2[e/x]$ (rule format: $\frac{e_1[e/x]=a\ e_2[e/x]=b}{(e_1\ e_2)[e/x] = a\ b}$)
		
		Need to prove: $FV((e_1\ e_2)[e/x]) \subseteq (FV(e_1\ e_2) -\{x\}) \cup FV(e)$
		
		(1) $FV((e_1\ e_2)[e/x]) = FV(e_1[e/x]) \cup FV(e_2[e/x])$ (by assumption)
		
		(2) $FV(e_1[e/x]) \subseteq (FV(e_1) -\{x\}) \cup FV(e)$ (by I.H.)
		
		(3) $FV(e_2[e/x]) \subseteq (FV(e_2) -\{x\}) \cup FV(e)$ (by I.H.)
		
		(4) $FV((e_1\ e_2)[e/x]) \subseteq (FV(e_1) -\{x\}) \cup (FV(e_2) -\{x\}) \cup FV(e) \subseteq (FV(e_1\ e_2) -\{x\}) \cup FV(e)$ (by (1), (2) and (3))
		
		\item case $(\lambda x.e_1)[e/x] = \lambda x.e_1$
		
		Need to prove $FV((\lambda x.e_1)[e/x]) \subseteq (FV(\lambda x.e_1) -\{x\}) \cup FV(e)$
		
		(1) $FV((\lambda x.e_1)[e/x]) = FV(\lambda x.e_1)$ (by assumption)
		
		(2) $FV((\lambda x.e_1)[e/x]) \subseteq (FV(\lambda x.e_1) -\{x\}) \cup FV(e)$ (by (1))
		
		\item case $(\lambda y.e_1)[e/x] = \lambda y.(e_1[e/x])$ ($y \neq x$ and $y \notin FV(e)$)
		
		Need to prove $FV((\lambda y.e_1)[e/x]) \subseteq (FV(\lambda y.e_1) -\{x\}) \cup FV(e)$
		
		(1) $FV((\lambda y.e_1)[e/x]) = FV(\lambda y.(e_1[e/x])) = FV(e_1[e/x]) - \{y\}$ (by assumption)
		
		(2) $FV(e_1[e/x]) \subseteq (FV(e_1) - \{x\}) \cup FV(e)$ (by I.H.)
		
		(3) $FV(\lambda y.e_1) = FV(e_1) -\{y\}$
		
		(4) $FV((\lambda y.e_1)[e/x]) \subseteq (FV(\lambda y.e_1) -\{x\}) \cup FV(e)$ (by (1), (2) and (3))
		
		\item case $(\lambda y.e_1)[e/x] = \lambda z.(e_1[[z/y]][e/x])$ ($y \neq x$, $y \in FV(e)$ and $z \notin FV(e) \cup Vars(e_1)$)
		
		Need to prove $FV((\lambda y.e_1)[e/x]) \subseteq (FV(\lambda y.e_1) -\{x\}) \cup FV(e)$
		
		(1) $FV((\lambda y.e_1)[e/x]) = FV(\lambda z.(e_1[[z/y]][e/x])) = FV(e_1[[z/y]][e/x]) - \{z\}$ (by assumption)
		
		(2) $FV(e_1[[z/y]][e/x]) \subseteq (FV(e_1[[z/y]]) - \{x\}) \cup FV(e)$ (by I.H.)
		
		(3) $FV(e_1[[z/y]]) \subseteq (FV(e_1) - \{y\}) \cup FV(z)$ (by I.H.)
		
		(4) $FV(\lambda y.e_1) = FV(e_1) - \{y\}$
		
		(5) $FV((\lambda y.e_1)[e/x]) \subseteq (FV(\lambda y.e_1) -\{x\}) \cup FV(e)$ (by (1), (2), (3) and (4))
		
	\end{enumerate}
\end{proof}
About the proof of this Lemma, you just need to know the idea. I found another proof ( \href{https://www.cs.bham.ac.uk/research/projects/poplog/paradigms_lectures/lambda_calculus_html.d/substitution.html}{This is another proof}) from the internet. You will find the idea is the same. Both proofs use induction to prove this property.


\end{document}